finish verification of reduce kernel on sequencial semantics

fold.v
@@ -14,6 +14,7 @@ Notation T1 := (Var 4).
 Notation T2 := (Var 5).
 Notation ARR := (Var 6).
 Notation SARR := (Var 7).
+Notation OUT := (Var 8).
 
 Definition If (b : bexp) (c : cmd) := Cif b c.
 
@@ -29,9 +30,10 @@ Variable f : nat -> Z.
 
 Notation f_ss := (skip_sum nt_gr 0 len f).
 
-Definition INV2 i :=
+Definition INV2 i b :=
   Ex (s e : nat) fc,
     !(TID === Enum' i) **
+    !(BID === Enum' b) **
     !(St === Enum' s) **
     !(pure (s = (2 ^ e / 2))) **
     !(pure (if lt_dec i (ceil2 s) then
@@ -44,23 +46,24 @@ Definition INV2 i :=
      else
        nth i (distribute s (Sh SARR) ntrd fc (nt_step s) 0) emp).
 
-Definition INV1 tid1 tid2 :=
+Definition INV1 i b :=
   Ex (ix : nat) (v : Z),
-    !(TID === Enum' tid1) **
-    !(I === Enum' (ix * nt_gr + tid2)) **
-    !(Apure (ix * nt_gr + tid2 < len + nt_gr)%nat) **
-    !(T2 === skip_sum nt_gr 0 (ix * nt_gr) f tid2) **
-    skip_arr (Gl ARR) 0 len nt_gr f tid2 **
-    (Sh SARR +o Enum' tid1 -->p (1%Qc, v)).
+    !(TID === Enum' i) **
+    !(BID === Enum' b) **
+    !(I === Enum' (ix * nt_gr + (i + b * ntrd))) **
+    !(Apure (ix * nt_gr + (i + b * ntrd) < len + nt_gr)%nat) **
+    !(T2 === skip_sum nt_gr 0 (ix * nt_gr) f (i + b * ntrd)) **
+    skip_arr (Gl ARR) 0 len nt_gr f (i + b * ntrd) **
+    (Sh SARR +o Enum' i -->p (1%Qc, v)).
 
 Open Scope bexp_scope.
 
 Close Scope bexp_scope.
-Definition fold_ker (i1 i2 : nat) :=
+Definition fold_ker (i b : nat) := (
   I ::= (TID +C BID *C Z.of_nat ntrd) ;;
   T2 ::= [ Gl ARR +o I ] ;;
   I ::= I +C Z.of_nat ntrd *C Z.of_nat nblk ;;
-  WhileI (INV1 i1 i2) ( I <C Z.of_nat len ) (
+  WhileI (INV1 i b) ( I <C Z.of_nat len ) (
     T1 ::= [ Gl ARR +o I ] ;;
     T2 ::= T1 +C T2 ;;
     I ::= Z.of_nat ntrd *C Z.of_nat nblk + I
@@ -68,15 +71,19 @@ Definition fold_ker (i1 i2 : nat) :=
   [ Sh SARR +o TID ] ::= T2 ;;
   Cbarrier 0;;
   St ::= Enum' ntrd >>1;;
-  WhileI (INV2 i1) ( Enum' 0 < St ) (
+  WhileI (INV2 i b) ( Enum' 0 < St ) (
     If ( Evar TID <C St ) (
-      T1 ::= [ Gl ARR +o TID ] ;;
-      T2 ::= [ Gl ARR +o (TID + St) ] ;;
-      [ Gl ARR +o TID ] ::= T1 + T2
+      T1 ::= [ Sh SARR +o TID ] ;;
+      T2 ::= [ Sh SARR +o (TID + St) ] ;;
+      [ Sh SARR +o TID ] ::= T1 + T2
     ) (SKIP) ;;
     St ::= St >>1 ;;
-    Cbarrier 0
-  )%exp.
+    Cbarrier 1
+  );;
+  If (TID == 0%Z) (
+    T1 ::= [ Sh SARR +o 0%Z] ;;
+    [ Gl OUT +o BID ] ::= T1
+  ) SKIP)%exp.
 
 Definition fold_ker' : cmd := fold_ker 0 0.
 
@@ -88,26 +95,30 @@ Definition binv0 (bid : Fin.t nblk) : Vector.t assn ntrd * Vector.t assn ntrd :=
    let tid := nf i in
    nth tid (distribute (ceil2 (ntrd /2)) (Sh SARR) ntrd f_ss (nt_step (ceil2 (ntrd / 2))) 0) emp)).
    
-Definition binv1 : Vector.t assn ntrd * Vector.t assn ntrd :=
+Definition binv1 (b : Fin.t nblk) : Vector.t assn ntrd * Vector.t assn ntrd :=
   (MyVector.init (fun i : Fin.t ntrd =>
    let tid := nat_of_fin i in
-   Ex s fc,
+   Ex s e fc,
      !(St === Enum' s) **
-      let tid := nat_of_fin i in
-      !(pure (if lt_dec tid (dbl s) then fc tid = skip_sum (dbl s) 0 ntrd f tid else True)) **
-      nth tid (distribute (dbl s) (Gl ARR) ntrd fc (nt_step (dbl s)) 0) emp **
-      !(pure (dbl s <= ntrd / 2))),
+     !(pure (s = (2 ^ e / 2))) **
+     let tid := nat_of_fin i in
+     !(pure (if lt_dec tid (dbl s) then fc tid = skip_sum (dbl s) 0 ntrd f_ss tid else True)) **
+     nth tid (distribute (dbl s) (Sh SARR) ntrd fc (nt_step (dbl s)) 0) emp **
+     !(pure (s <= ntrd / 2)) **
+     !(BID === Enum' (nf b))),
    MyVector.init (fun i => 
    let tid := nat_of_fin i in
-   Ex s fc, 
+   Ex s e fc, 
      !(St === Enum' s) **
-      let tid := nat_of_fin i in
-      !(pure (if lt_dec tid (ceil2 s) then
-                fc tid = skip_sum (dbl s) 0 ntrd f tid /\
-                fc (tid + s) = skip_sum (dbl s) 0 ntrd f (tid + s)
-              else True)) **
-      nth tid (distribute (ceil2 s) (Gl ARR) ntrd fc (nt_step (ceil2 s)) 0) emp **
-      !(pure (dbl s <= ntrd / 2)))).
+     !(pure (s = (2 ^ e / 2))) **
+     let tid := nat_of_fin i in
+     !(pure (if lt_dec tid (ceil2 s) then
+               fc tid = skip_sum (dbl s) 0 ntrd f_ss tid /\
+               fc (tid + s) = skip_sum (dbl s) 0 ntrd f_ss (tid + s)
+             else True)) **
+     nth tid (distribute (ceil2 s) (Sh SARR) ntrd fc (nt_step (ceil2 s)) 0) emp **
+     !(pure (s <= ntrd / 2)) **
+     !(BID === Enum' (nf b)))).
 
 Arguments div _ _ : simpl never.
 Lemma nf_lt (n : nat) (i : Fin.t n) : nf i < n.
@@ -132,22 +143,42 @@ Qed.
 Hint Resolve nf_lt.
 Hint Resolve nt_gr_neq_0 id_lt_nt_gr nf_lt.
 
+Lemma rule_frame' (ntrd' : nat) (bspec : nat -> Vector.t assn ntrd' * Vector.t assn ntrd')
+      (tid : Fin.t ntrd') (C : cmd) (P Q R : assn) :
+  CSL bspec tid P C Q ->
+  inde R (writes_var C) -> CSL bspec tid (R ** P) C (R ** Q).
+Proof.
+  intros.
+  eapply Hbackward; [eapply Hforward|].
+  apply rule_frame.
+  apply H.
+  apply H0.
+  intros; repeat sep_cancel.
+  intros; repeat sep_cancel.
+Qed.
+
+Definition binv bid i :=
+  if Nat.eq_dec i 0 then binv0 bid else if Nat.eq_dec i 1 then binv1 bid else default ntrd.
+
 Theorem fold_ker_correct (tid : Fin.t ntrd) (bid : Fin.t nblk) :
   nt_gr <= len ->
-  CSL (fun i => match i with O => binv0 bid | _ => default ntrd end) tid
-  (Ex  (v : Z),
-   (Sh SARR +o Z_of_fin tid -->p (1, v)) **
+  CSL (binv bid) tid
+  (Ex  (v1 v2 : Z),
+   (Sh SARR +o Z_of_fin tid -->p (1, v1)) **
    skip_arr (Gl ARR ) 0 len        nt_gr f  (nf tid + nf bid * ntrd) **
+   (if Nat.eq_dec (nf tid) 0 then (Gl OUT +o Z_of_fin bid -->p (1, v2)) else emp) **
    !(TID === Z_of_fin tid) **
    !(BID === Z_of_fin bid))
-  (fold_ker (nf tid) (nf tid + nf bid * ntrd))
+  (fold_ker (nf tid) (nf bid))
   (Ex fc,
-     nth (nat_of_fin tid) (distribute 1 (Gl ARR) (ntrd * 2) fc (nt_step 1) 0) emp **
      skip_arr (Gl ARR ) 0 len        nt_gr f (nf tid + nf bid * ntrd) **
-     !(pure (if Nat.eq_dec (nf tid) 0 then (fc 0 = sum_of 0 (ntrd * 2) f) else True))).
+     if Nat.eq_dec (nf tid) 0 then
+       nth (nat_of_fin tid) (distribute 1 (Sh SARR) ntrd fc (nt_step 1) 0) emp **
+       (Gl OUT +o Z_of_fin bid -->p (1, sum_of 0 ntrd f_ss))
+     else emp).
 Proof.
   intros Hnlen.
-  unfold fold_ker, skip_arr.
+  unfold fold_ker, skip_arr, binv.
   pose proof (nf_lt tid) as nf_lt.
   assert (Hnt_gr : nf tid + nf bid * ntrd < nt_gr) by eauto.
   repeat hoare_forward.
@@ -180,7 +211,12 @@ Proof.
   { hoare_forward. intros ? ? [v H]. subA_normalize_in H. simpl in H.
     ex_intro v H; exact H. }
 
+  hoare_forward.
+  eapply Hbackward.
+  Focus 2. { intros ? ? H. sep_normal_in H. sep_lift_in H 7. exact H. } Unfocus.
   eapply rule_seq.
+  apply rule_frame'.
+  2: prove_inde.
   { repeat hoare_forward; unfold INV1, skip_arr.
     - { eapply Hbackward.
         Focus 2. {
@@ -205,23 +241,57 @@ Proof.
       { hoare_forward; intros ? ? [v H]. subA_normalize_in H. simpl in H. ex_intro v H; exact H. }
       repeat hoare_forward. intros ? ? [v H].
       subA_normalize_in H. simpl in H.
-      sep_normal_in H; sep_split_in H.
+      sep_normal_in H. sep_split_in H.
       unfold_pures. subst v.
-      exists (S x2) x1.
+      exists (S x3) x2.
       sep_split; eauto.
       - unfold_conn; simpl; nia.
       - unfold_conn; simpl. nia.
-      - unfold_conn; simpl. admit.
-      - sep_rewrite (@skip_arr_nth' x2); [|first [now eauto | omega | nia]..].
+      - unfold_conn; simpl.
+        Lemma skip_sum_app sk ix (f' : nat -> Z) i : 
+          sk <> 0 -> i < sk -> forall st,
+          skip_sum sk (st * sk) (sk + ix * sk) f' i =
+          (f' (i + ix * sk + st * sk)%nat + skip_sum sk (st * sk) (ix * sk) f' i)%Z.
+        Proof.
+          intros Hsk Hisk; induction ix; simpl; intros st.
+          - rewrite <-!plus_n_O, Z.add_0_r.
+            rewrite skip_sum_unfold; eauto.
+            rewrite minus_diag; simpl; omega.
+          - rewrite skip_sum_unfold; try nia.
+            rewrite (skip_sum_unfold (len := sk + ix * sk)); try nia.
+            cutrewrite (sk + (sk + ix * sk) - sk = sk + ix * sk); [|nia].
+            rewrite IHix.
+            ring_simplify.
+            cutrewrite (i + (sk + ix * sk) + st * sk = i + ix * sk + S st * sk); [|nia].
+            cutrewrite (sk + ix * sk - sk = ix * sk); [|nia]; eauto.
+        Qed.
+
+        Lemma skip_sum_app0 sk ix f' i :
+          sk <> 0 -> i < sk ->
+          skip_sum sk 0 (sk + ix * sk) f' i =
+          (f' (i + ix * sk)%nat + skip_sum sk 0 (ix * sk) f' i)%Z.
+        Proof.
+          intros; cutrewrite (0 = 0 * sk); eauto.
+          rewrite skip_sum_app; try omega.
+          simpl; rewrite <-plus_n_O; auto.
+        Qed.
+        subst. rewrite skip_sum_app0; try omega; eauto.
+        cutrewrite (nf tid + nf bid * ntrd + x3 * nt_gr = x3 * nt_gr + (nf tid + nf bid * ntrd));
+          [|ring].
+        nia.
+      - sep_rewrite (@skip_arr_nth' x3); [|first [now eauto | omega | nia]..].
         sep_normal; sep_normal_in H.
         repeat sep_cancel. }
     - intros ? ? H; exact H.
-    - intros s h H; sep_normal_in H; sep_split_in H; unfold_pures. subst x0.
+    - intros s h H; sep_normal_in H; sep_split_in H; unfold_pures. subst x1.
       exists 1 x.
       sep_split; eauto.
       + unfold_conn; simpl. nia.
       + unfold_conn; simpl. nia.
-      + unfold_conn; simpl. admit.
+      + unfold_conn; simpl.
+        rewrite <-plus_n_O.
+        cutrewrite (0 = 0 * nt_gr); eauto; rewrite skip_sum_unfold; try omega; eauto.
+        autorewrite with sep; eauto.
       + assert (Heq : 0 = 0 * nt_gr) by auto; rewrite Heq; clear Heq.
         sep_rewrite skip_arr_unfold'; try nia.
         simpl.
@@ -232,12 +302,14 @@ Proof.
   { eapply Hbackward.
     Focus 2. {
     intros ? ? H.
-    apply ex_lift_l_in in H; destruct H as [ix H].
-    apply ex_lift_l_in in H; destruct H as [v H].
+    sep_split_in H.
+    apply ex_lift_r_in in H; destruct H as [ix H].
+    apply ex_lift_r_in in H; destruct H as [v H].
     sep_normal_in H.
+    sep_combine_in H.
     ex_intro v H. ex_intro ix H. simpl in H. exact H. } Unfocus.
     repeat hoare_forward.
-    intros ? ? H. ex_intro x0 H. exact H. }
+    intros ? ? H. ex_intro x2 H. exact H. }
 
   hoare_forward.
   eapply rule_seq.
@@ -245,16 +317,90 @@ Proof.
     intros s h H; exact H.
     intros s h H. simpl. rewrite MyVector.init_spec.
     sep_split_in H.
-    assert (Heq : skip_sum nt_gr 0 (x0 * nt_gr) f (nf tid + nf bid * ntrd) =
-                  f_ss (nf tid + nf bid * ntrd)) by admit.
-    rewrite Heq in HP2.
-    change_in H.
-    { clear HP0 HP1 HP2 HP3.
-      sep_combine_in H. exact H. }
-    sep_cancel. }
+    assert (Heq : skip_sum nt_gr 0 (x2 * nt_gr) f (nf tid + nf bid * ntrd) =
+                  f_ss (nf tid + nf bid * ntrd)).
+    { unfold_pures.
+      assert (len <= x2 * nt_gr + (nf tid + nf bid * ntrd)) by nia.
 
+      Lemma skip_sum_nil' next sk len1 f1 i : forall st,
+        (forall j, j < next -> (st + len1 + j) mod sk <> i) ->
+        skip_sum sk st len1 f1 i =
+        skip_sum sk st (len1 + next) f1 i.
+      Proof.
+        induction len1; intros st Hst; simpl.
+        - rewrite (@skip_sum_nil next).
+          { rewrite minus_diag; eauto. }
+          rewrite <-plus_n_O in Hst; eauto.
+        - rewrite IHlen1; eauto.
+          intros; cutrewrite (S st + len1 + j = st + S len1 + j); [|nia]; eauto.
+      Qed.
+      Lemma mod_lt n m a b : m <> 0 ->
+        n * m <= a < b -> b < (S n) * m ->
+        a mod m < b mod m.
+      Proof.
+        intros Hm0 Ha Hb; destruct Ha.
+        assert (a / m = n).
+        { apply (Nat.div_le_mono _ _ m) in H; try omega.
+          rewrite Nat.div_mul in H; try omega.
+          assert (a < S n * m) by omega.
+          rewrite mult_comm in H1; apply Nat.div_lt_upper_bound in H1; omega. }
+        assert (b / m = n).
+        { assert (n * m <= b) by omega.
+          apply (Nat.div_le_mono _ _ m) in H2; try omega.
+          rewrite Nat.div_mul in H2; try omega.
+          rewrite mult_comm in Hb; apply Nat.div_lt_upper_bound in Hb; try omega. }
+        rewrite (Nat.div_mod a m), (Nat.div_mod b m) in H0; try omega.
+        rewrite H1, H2 in H0; omega.
+      Qed.
+      Lemma mod_le n m a b : m <> 0 ->
+        n * m <= a <= b -> b < (S n) * m ->
+        a mod m <= b mod m.
+      Proof.
+        intros Hm0 Ha Hb; destruct Ha.
+        assert (a / m = n).
+        { apply (Nat.div_le_mono _ _ m) in H; try omega.
+          rewrite Nat.div_mul in H; try omega.
+          assert (a < S n * m) by omega.
+          rewrite mult_comm in H1; apply Nat.div_lt_upper_bound in H1; omega. }
+        assert (b / m = n).
+        { assert (n * m <= b) by omega.
+          apply (Nat.div_le_mono _ _ m) in H2; try omega.
+          rewrite Nat.div_mul in H2; try omega.
+          rewrite mult_comm in Hb; apply Nat.div_lt_upper_bound in Hb; try omega. }
+        rewrite (Nat.div_mod a m), (Nat.div_mod b m) in H0; try omega.
+        rewrite H1, H2 in H0; omega.
+      Qed.
+
+      assert (len < x2 * nt_gr \/ x2 * nt_gr <= len) as [Hl | Hl ] by omega.
+      - rewrite (@skip_sum_nil' (x2 * nt_gr - len) _ len).
+        cutrewrite (len + (x2 * nt_gr - len) = x2 * nt_gr); [|nia]; eauto.
+        intros j Hj; simpl.
+        assert (len <= len + j < x2 * nt_gr) by omega.
+        assert ((x2 - 1) * nt_gr + (nf tid + nf bid * ntrd) < len) by nia.
+        assert (len mod nt_gr <= (len + j) mod nt_gr).
+        { apply (@mod_le (x2 - 1)); eauto; try omega; nia. }
+        assert (((x2 - 1) * nt_gr + (nf tid + nf bid * ntrd)) mod nt_gr < len mod nt_gr).
+        { apply (@mod_lt (x2 - 1)); eauto; try omega; nia. }
+        rewrite plus_comm, Nat.mod_add, Nat.mod_small in H4; omega.
+      - rewrite (@skip_sum_nil' (len - x2 * nt_gr) _ (x2 * nt_gr)).
+        cutrewrite (x2 * nt_gr + (len - x2 * nt_gr) = len); [|omega]; auto.
+        intros j Hj; simpl.
+        assert (nf tid + nf bid * ntrd < nt_gr) by eauto.
+        assert (len < S x2 * nt_gr) by nia.
+        assert (x2 *nt_gr + j < len) by nia.
+        assert ((x2 * nt_gr + j) mod nt_gr < len mod nt_gr).
+        { apply (@mod_lt x2); eauto; try omega; nia. }
+        assert (len mod nt_gr <= (x2 * nt_gr + (nf tid + nf bid * ntrd)) mod nt_gr).
+        { apply (@mod_le x2); eauto; try omega; nia. }
+        rewrite plus_comm, Nat.mod_add, (Nat.mod_small (nf tid + nf bid * ntrd)) in H5; try omega.
+    }
+        rewrite Heq in HP4.
+        change_in H.
+        { clear HP HP2 HP3 HP4; 
+          sep_combine_in H. exact H. }
+        sep_cancel. }
+    
   (* introduction *)
-  unfold fold_ker.
   (* assert (Htid : nat_of_fin tid < ntrd) by (destruct (Fin.to_nat tid); simpl in *; try omega). *)
   (* remember (ntrd * 2) eqn:Hntrd2. *)
 
@@ -264,6 +410,26 @@ Proof.
     simpl; intros ? ? [v H].
     eapply scRw in H; [|intros ? ? H'; subA_normalize_in H'; exact H' | intros ? ? H'; exact H'].
     simpl in H; exact H. }
+
+  (* frame out irrelevant resources *)
+  eapply rule_seq.
+  eapply Hbackward.
+  Focus 2. {
+    intros ? ? H. sep_normal_in H.
+    sep_lift_in H 3.
+    exact H.
+  } Unfocus.
+  apply rule_frame'.
+  2: prove_inde.
+
+  eapply Hbackward.
+  Focus 2. {
+    intros ? ? H. sep_normal_in H.
+    sep_lift_in H 3.
+    exact H.
+  } Unfocus.
+  apply rule_frame'.
+  2: prove_inde.  
 
   (* the loop invariant holds before the loop *)
   hoare_forward.
@@ -294,12 +460,12 @@ Proof.
         cutrewrite (2 ^ S e = 2 ^ e * 2); [|simpl; omega].
         rewrite Nat.mod_mul; eauto.
     - red; auto.
-    - unfold ceil2 in *. destruct (Nat.eq_dec _ _). [omega | congruence]. } Unfocus.
+    - unfold ceil2 in *. destruct (Nat.eq_dec _ _); eauto. } Unfocus.
 
   (* make the precondition normal form *)
   eapply Hbackward.
   Focus 2.
-  { unfold INV; intros s h H.
+  { unfold INV2; intros s h H.
     sep_split_in H; destruct H as (st & e & fc & H).
     sep_combine_in H.
     ex_intro st H; ex_intro e H; ex_intro fc H.
@@ -314,7 +480,7 @@ Proof.
   { eapply Hbackward.
     Focus 2.
     (* unfold the skip array *) 
-    { unfold INV; intros s h H.
+    { unfold INV2; intros s h H.
       sep_split_in H.
       change_in H.
       { unfold_pures.
@@ -322,8 +488,13 @@ Proof.
         cutrewrite (0 = 0 * st) in H; [|auto].
         apply skip_arr_unfold' in H; simpl; try omega; simpl in H.
         cutrewrite (st + 0 = 1 * st) in H; [|omega].
-        sep_rewrite_in skip_arr_unfold' H; try omega.
-        rewrite mult_1_l in H; exact H. }
+        sep_rewrite_in skip_arr_unfold' H; try first [omega].
+        rewrite mult_1_l in H; exact H.
+        assert (st + st <= ntrd / 2 + ntrd / 2) by omega.
+        assert (ntrd / 2 + ntrd / 2 <= ntrd).
+        { pose proof (@div_mult ntrd 2); omega. }
+        assert (nf tid < st) by nia.
+        omega. }
       sep_combine_in H.
       exact H. } Unfocus.
 
@@ -374,7 +545,7 @@ Proof.
 
     (* the barrier instruction *)
     hoare_forward.
-    instantiate (1 := INV (nf tid)).
+    instantiate (1 := INV2 (nf tid) (nf bid)).
     set (fc' := (fun i => if Nat.eq_dec i (nf tid) then (fc i + fc (i + st)%nat)%Z else fc i)).
     destruct e as [|e].
 
@@ -382,86 +553,156 @@ Proof.
       forward_barr. Focus 2.
       { simpl; rewrite MyVector.init_spec.
         intros s h H; sep_normal_in H; sep_split_in H.
-        unfold_conn_in (HP3, HP4, HP5); simpl in HP3, HP4, HP5.
+        unfold_conn_in (HP3, HP5, HP6); simpl in HP3, HP5, HP6.
         assert (FalseP s h) by (subst; simpl in HP3; congruence). 
         instantiate (1 := FalseP). destruct H0. } Unfocus.
       intros; unfold_conn; repeat destruct H; tauto.
 
     + (* fold skip array *)
-      eapply Hbackward. Focus 2.
-      { intros s h H; sep_split_in H.
-        assert ((T1 + T2 === (fc (nf (tid)) + fc (st + nf tid)%nat)%Z) s (emp_ph loc)) by
-            (unfold_conn_all; simpl in *; omega).
-        fold (2 ^ S (S e) / 2) in *.
-        assert (Hst : st = 2 ^ (S e) / 2) by (unfold_conn_in HP6; auto).
-        cutrewrite (2 ^ (S e) = 2 ^ e * 2) in Hst; [|simpl; omega].
-        rewrite Nat.div_mul in Hst; auto.
-        sep_rewrite_in mps_eq2 H; [|exact H0].
+      forward_barr.
+      Focus 2.
+      { rewrite pow_divS; eauto. simpl; rewrite MyVector.init_spec.
+        intros s h H.
+        apply ex_lift_l. exists (st / 2).
+        apply ex_lift_l. exists e.
+        apply ex_lift_l. exists fc'.
+        instantiate (1 := !(TID === Zn (nf tid))).
+        sep_normal; sep_split_in H; sep_split; eauto.
+        - unfold_pures.
+          autorewrite with sep in *; eauto. unfold_conn; simpl. congruence.
+        - unfold_pures. 
+        - unfold_pures; unfold fc'; unfold_conn; simpl; subst st.
+          autorewrite with sep in *.
+          destruct lt_dec; eauto.
+          destruct Nat.eq_dec; try congruence.
+          destruct HP8 as [Heq Heq']; rewrite Heq, Heq'; clear Heq Heq'.
+          cutrewrite (2 ^ S e = 2 ^ e * 2); [|simpl; omega].
+          lets Heq: (>>skip_sum_double (2 ^ e) (nf tid) ntrd 0); eauto.
+        - unfold_pures; unfold fc'; unfold_conn; simpl; subst st.
+          Lemma div_le a b: b <> 0 -> a / b <= a.
+          Proof.
+            intros.
+            lets: (Nat.div_le_compat_l a 1 b).
+            rewrite Nat.div_1_r in H0.
+            apply H0; omega.
+          Qed.
+          lets: (>>div_le (2 ^ e) 2); omega.
+        (* - unfold_pures; unfold fc'; unfold_conn; simpl; subst st. *)
+        (*   autorewrite with sep in *; eauto. *)
+        - unfold_pures.
+          assert (Heq : dbl (st / 2) = st).
+          { unfold_pures; unfold fc'; unfold_conn; simpl; subst st; autorewrite with sep; auto. }
+          rewrite Heq.
+          assert (st <> 0).
+          { unfold_pures; subst st; eauto. }
+          assert (nf tid < st).
+          { unfold_pures; subst. nia. }
+          cutrewrite (0 = 0 * st); eauto.
+          sep_rewrite skip_arr_unfold'; try omega.
+          sep_rewrite skip_arr_unfold'; try first [omega].
+          sep_normal.
+          unfold fc'.
+          destruct Nat.eq_dec; try omega.
+          destruct Nat.eq_dec; try omega.
+          sep_cancel.
+          cutrewrite (0 * st + nf tid + st = st + nf tid); [|ring].
+          sep_cancel.
+          rewrite !Nat2Z.inj_add, Nat2Z.inj_mul.
+          cutrewrite (1 * st + nf tid = st + nf tid); [|ring].
+          cutrewrite (Zn 1 * Zn st = Zn st)%Z; [|ring].
+          sep_cancel.
+          sep_rewrite (nth_dist_change); try omega; eauto.
+          intros j Hj Hlt.
+          destruct Nat.eq_dec; try omega.
+          cut (nf tid + st < ntrd); [omega|].
+          assert (ntrd / 2 + ntrd / 2 <= ntrd).
+          { lets: (@div_mult ntrd 2); try omega. }
+          omega. } Unfocus.
 
-        assert (nf tid < st)
-          by (unfold_conn_all; simpl in *; destruct (Z_lt_dec (s TID) x); (congruence||omega)).
-        sep_rewrite_in (@nth_dist_change (nat_of_fin tid) (Gl ARR) fc fc') H;
-          try now (subst; auto || unfold_conn_all; simpl in *; omega).
-        2 : rewrite <-!plus_n_O; intros; unfold fc'; destruct Nat.eq_dec; auto; omega.
-        cutrewrite (st + (st + 0) = 2 * st) in H; [|omega].
-        assert ((Gl ARR +o (TID + x) ===l Gl ARR +o Z.of_nat (1 * st + nf tid))%exp s (emp_ph loc)).
-        { unfold_conn_all; simpl; simplify_loc; rewrite !Nat2Z.inj_add, Z.add_0_r; simpl in*; omega. }
-        sep_rewrite_in (@mps_eq1 (Gl ARR +o (TID + x))%exp ) H; [|exact H2].
-        cutrewrite (fc (nf tid) + fc (st + nf tid)%nat = fc' (0 * st + nf tid)%nat)%Z in H; [|].
-        2: unfold fc'; destruct Nat.eq_dec; unfold_conn_all; simpl in *; [f_equal; f_equal; omega| omega].
-        cutrewrite (fc (st + nf tid)%nat = fc' (1 * st + nf tid)%nat)%Z in H; [|].
-        2: unfold fc'; destruct Nat.eq_dec; unfold_conn_all; simpl in *; [omega|f_equal; omega].
-        sep_rewrite_in_r skip_arr_unfold' H; (omega || auto).
-        2: unfold_conn_in HP8; omega.
-        assert ((Gl (ARR + TID)%exp ===l Gl ARR +o Z.of_nat (0 * st + nf tid)) s (emp_ph loc)).
-        { unfold_conn_all; simpl in *; simplify_loc; omega. }
-        sep_rewrite_in mps_eq1 H; [|exact H3].
-        sep_rewrite_in_r skip_arr_unfold' H; (omega || auto).
-        clear HP0 HP1 HP2 H0.
-        sep_combine_in H. exact H. } Unfocus.
+      intros ? ? H.
+      apply ex_lift_l_in in H as [st' H].
+      apply ex_lift_l_in in H as [e' H].
+      apply ex_lift_l_in in H as [fc0 H].
+      sep_normal_in H; sep_split_in H; unfold_pures; unfold INV2.
+      exists st' e' fc0; sep_split; eauto.
+      unfold ceil2 in *.
+      destruct Nat.eq_dec; eauto.
 
-      (* barrier pre holds at barrier (then) *)
-      forward_barr. Focus 2.
-      { autorewrite with sep; auto.
-        simpl; rewrite MyVector.init_spec. 
-        intros s h H; sep_normal_in H; sep_split_in H.
-        apply ex_lift_l; exists (2 ^ e / 2); apply ex_lift_l; exists fc'.
-        do 3 (sep_normal; sep_split).
-        - unfold_pures. autorewrite with sep in *; auto; simpl. 
-          unfold_conn; simpl; congruence.
-        - unfold_pures; unfold_conn; autorewrite with sep in *.
-          unfold fc' in *; clear fc'; subst st; rewrite ceil2_pow in HP4.
-          destruct Nat.eq_dec; try omega; destruct (lt_dec); auto.
-          destruct HP4 as [Heq1 Heq2]; rewrite Heq1, Heq2; autorewrite with sep.
-          cutrewrite (2 ^ S e = 2^e*2); [|simpl; omega].
-          cutrewrite (0 = 0 * 2 * (2^e * 2)); [|omega]; apply (skip_sum_double) ; omega.
-        - rewrite dbl_inv.
-          unfold_conn_all; simpl in *; omega.
-        - sep_normal. 
-          rewrite dbl_inv.
-          cutrewrite (2 ^ e = st); [|unfold_conn_all; congruence].
-          sep_combine_in H; sep_cancel. exact H. } Unfocus.
+      (* eapply Hbackward. Focus 2. *)
+      (* { intros s h H; sep_split_in H. *)
+      (*   assert ((T1 + T2 === (fc (nf (tid)) + fc (st + nf tid)%nat)%Z) s (emp_ph loc)) by *)
+      (*       (unfold_conn_all; simpl in *; omega). *)
+        
+      (*   fold (2 ^ S (S e) / 2) in *. *)
+      (*   assert (Hst : st = 2 ^ (S e) / 2) by (unfold_conn_in HP6; auto). *)
+      (*   cutrewrite (2 ^ (S e) = 2 ^ e * 2) in Hst; [|simpl; omega]. *)
+      (*   rewrite Nat.div_mul in Hst; auto. *)
+      (*   sep_rewrite_in mps_eq2 H; [|exact H0]. *)
+
+      (*   assert (nf tid < st) *)
+      (*     by (unfold_conn_all; simpl in *; destruct (Z_lt_dec (s TID) x); (congruence||omega)). *)
+      (*   sep_rewrite_in (@nth_dist_change (nat_of_fin tid) (Gl ARR) fc fc') H; *)
+      (*     try now (subst; auto || unfold_conn_all; simpl in *; omega). *)
+      (*   2 : rewrite <-!plus_n_O; intros; unfold fc'; destruct Nat.eq_dec; auto; omega. *)
+      (*   cutrewrite (st + (st + 0) = 2 * st) in H; [|omega]. *)
+      (*   assert ((Gl ARR +o (TID + x) ===l Gl ARR +o Z.of_nat (1 * st + nf tid))%exp s (emp_ph loc)). *)
+      (*   { unfold_conn_all; simpl; simplify_loc; rewrite !Nat2Z.inj_add, Z.add_0_r; simpl in*; omega. } *)
+      (*   sep_rewrite_in (@mps_eq1 (Gl ARR +o (TID + x))%exp ) H; [|exact H2]. *)
+      (*   cutrewrite (fc (nf tid) + fc (st + nf tid)%nat = fc' (0 * st + nf tid)%nat)%Z in H; [|]. *)
+      (*   2: unfold fc'; destruct Nat.eq_dec; unfold_conn_all; simpl in *; [f_equal; f_equal; omega| omega]. *)
+      (*   cutrewrite (fc (st + nf tid)%nat = fc' (1 * st + nf tid)%nat)%Z in H; [|]. *)
+      (*   2: unfold fc'; destruct Nat.eq_dec; unfold_conn_all; simpl in *; [omega|f_equal; omega]. *)
+      (*   sep_rewrite_in_r skip_arr_unfold' H; (omega || auto). *)
+      (*   2: unfold_conn_in HP8; omega. *)
+      (*   assert ((Gl (ARR + TID)%exp ===l Gl ARR +o Z.of_nat (0 * st + nf tid)) s (emp_ph loc)). *)
+      (*   { unfold_conn_all; simpl in *; simplify_loc; omega. } *)
+      (*   sep_rewrite_in mps_eq1 H; [|exact H3]. *)
+      (*   sep_rewrite_in_r skip_arr_unfold' H; (omega || auto). *)
+      (*   clear HP0 HP1 HP2 H0. *)
+      (*   sep_combine_in H. exact H. } Unfocus. *)
+
+      (* (* barrier pre holds at barrier (then) *) *)
+      (* forward_barr. Focus 2. *)
+      (* { autorewrite with sep; auto. *)
+      (*   simpl; rewrite MyVector.init_spec.  *)
+      (*   intros s h H; sep_normal_in H; sep_split_in H. *)
+      (*   apply ex_lift_l; exists (2 ^ e / 2); apply ex_lift_l; exists fc'. *)
+      (*   do 3 (sep_normal; sep_split). *)
+      (*   - unfold_pures. autorewrite with sep in *; auto; simpl.  *)
+      (*     unfold_conn; simpl; congruence. *)
+      (*   - unfold_pures; unfold_conn; autorewrite with sep in *. *)
+      (*     unfold fc' in *; clear fc'; subst st; rewrite ceil2_pow in HP4. *)
+      (*     destruct Nat.eq_dec; try omega; destruct (lt_dec); auto. *)
+      (*     destruct HP4 as [Heq1 Heq2]; rewrite Heq1, Heq2; autorewrite with sep. *)
+      (*     cutrewrite (2 ^ S e = 2^e*2); [|simpl; omega]. *)
+      (*     cutrewrite (0 = 0 * 2 * (2^e * 2)); [|omega]; apply (skip_sum_double) ; omega. *)
+      (*   - rewrite dbl_inv. *)
+      (*     unfold_conn_all; simpl in *; omega. *)
+      (*   - sep_normal.  *)
+      (*     rewrite dbl_inv. *)
+      (*     cutrewrite (2 ^ e = st); [|unfold_conn_all; congruence]. *)
+      (*     sep_combine_in H; sep_cancel. exact H. } Unfocus. *)
       
-      (* loop invariant is preserved *)
-      intros s h H; unfold INV; clear fc'.
-      apply ex_lift_l_in in H; destruct H as (s0 & H).
-      apply ex_lift_l_in in H; destruct H as (fc' & H); sep_split_in H.
-      exists (2 ^ e / 2), e, fc'.
-      assert ((St === Z.of_nat (2 ^ e / 2)) s (emp_ph loc)).
-      { unfold_conn_in (HP, HP2, HP3); simpl in HP2, HP3; rewrite HP2, HP3 in HP; simpl in HP.
-        rewrite Zdiv2_div in HP. rewrite div_Zdiv; auto. }
-      assert (s0 = 2 ^ e / 2).
-        { unfold_conn_in (HP8, H0); rewrite HP8 in H0; simpl in H0.
-          apply Nat2Z.inj in H0; auto. }
-      sep_split; try now (unfold_conn_all; (auto || omega)).
-      * unfold_conn_in (HP8, H0); rewrite HP8 in H0; simpl in H0; apply Nat2Z.inj in H0;
-        rewrite H0 in HP9.
-        apply HP9.
-      * unfold_conn_in (HP5, HP3); simpl in HP5, HP3; unfold_conn.
-        assert (2 ^ e <> 0) by (apply Nat.pow_nonzero; auto).
-        assert (2 ^ e / 2 < 2 ^ e) by (apply Nat.div_lt; omega).
-        omega.
-      * unfold ceil2 in H; destruct Nat.eq_dec; subst; destruct Nat.eq_dec; (omega || auto).
+      (* (* loop invariant is preserved *) *)
+      (* intros s h H; unfold INV; clear fc'. *)
+      (* apply ex_lift_l_in in H; destruct H as (s0 & H). *)
+      (* apply ex_lift_l_in in H; destruct H as (fc' & H); sep_split_in H. *)
+      (* exists (2 ^ e / 2), e, fc'. *)
+      (* assert ((St === Z.of_nat (2 ^ e / 2)) s (emp_ph loc)). *)
+      (* { unfold_conn_in (HP, HP2, HP3); simpl in HP2, HP3; rewrite HP2, HP3 in HP; simpl in HP. *)
+      (*   rewrite Zdiv2_div in HP. rewrite div_Zdiv; auto. } *)
+      (* assert (s0 = 2 ^ e / 2). *)
+      (*   { unfold_conn_in (HP8, H0); rewrite HP8 in H0; simpl in H0. *)
+      (*     apply Nat2Z.inj in H0; auto. } *)
+      (* sep_split; try now (unfold_conn_all; (auto || omega)). *)
+      (* * unfold_conn_in (HP8, H0); rewrite HP8 in H0; simpl in H0; apply Nat2Z.inj in H0; *)
+      (*   rewrite H0 in HP9. *)
+      (*   apply HP9. *)
+      (* * unfold_conn_in (HP5, HP3); simpl in HP5, HP3; unfold_conn. *)
+      (*   assert (2 ^ e <> 0) by (apply Nat.pow_nonzero; auto). *)
+      (*   assert (2 ^ e / 2 < 2 ^ e) by (apply Nat.div_lt; omega). *)
+      (*   omega. *)
+      (* * unfold ceil2 in H; destruct Nat.eq_dec; subst; destruct Nat.eq_dec; (omega || auto). *)
   - eapply Hbackward.
     Focus 2.
     { (* fold skip array to emp *)
@@ -487,68 +728,131 @@ Proof.
     { (* barrier pre holds at barrier (else) *)
       intros s h H; simpl; rewrite MyVector.init_spec.
       sep_normal_in H; sep_split_in H.
-      apply ex_lift_l; exists ((2 ^ e) / 2 / 2).
+      assert ((2 ^ e) / 2 = 2 ^ (e - 1)).
+      { unfold_pures; destruct e; [simpl in *; omega|].
+        cutrewrite (S e - 1 = e); [|omega].
+        autorewrite with sep; eauto. }
+      apply ex_lift_l; exists (2 ^ (e - 1) / 2).
+      apply ex_lift_l; exists (e - 1).
       apply ex_lift_l; exists fc.
       sep_rewrite_in_r emp_unit_r H; sep_split_in H.
-      do 3 sep_normal; sep_split.
-      unfold_conn_all; simpl in *; autorewrite with sep in *; auto.
-      - unfold_pures; destruct (lt_dec (nf tid) (dbl _)); unfold_conn; auto.
-        rewrite HP1 in *; rewrite <-Nat2Z.inj_lt in n0.
-        destruct e as [|e]; [cbv in l; inversion l|].
-        autorewrite with sep in l0; autorewrite with sep in n0; auto; omega.
+      instantiate (1 := !(TID === Zn (nf tid))).
+      sep_normal; sep_split;
+      try now (unfold_conn_all; simpl in *; autorewrite with sep in *; auto).
+      - rewrite <-H0; unfold_pures; autorewrite with sep in *; auto.
+      - unfold_pures.
+        rewrite H0 in *; autorewrite with sep in *.
+        destruct lt_dec; try omega; eauto.
+        (* unfold_pures; destruct (lt_dec (nf tid) (dbl _)); unfold_conn; auto. *)
+        (* rewrite HP1 in *; rewrite <-Nat2Z.inj_lt in n0. *)
+        (* destruct e as [|e]; [cbv in l; inversion l|]. *)
+        (* autorewrite with sep in l0; autorewrite with sep in n0; auto; omega. *)
       - unfold_pures; unfold_conn.
-        destruct e as [|e]; [cbv in l; inversion l|].
-        autorewrite with sep; auto. autorewrite with sep in HP4; auto.
-      - destruct e as [|e]; [unfold_pures; cbv in HP2; inversion HP2|].  
-        change_; [intros Hf|].
-        { autorewrite with sep in HP5; auto; unfold_pures.
-          rewrite HP1 in n0; rewrite <-Nat2Z.inj_lt in n0.
-          rewrite nth_overflow; [|rewrite distribute_length; autorewrite with sep in *; omega].
-          exact Hf. }
-        sep_combine_in H; sep_cancel; exact H. } Unfocus.
+        lets: (>>div_le (2 ^ (e - 1)) 2).
+        omega.
+      (* - unfold_pures; unfold_conn. *)
+      (*   destruct e as [|e]; [cbv in l; inversion l|]. *)
+      (*   autorewrite with sep; auto. autorewrite with sep in HP4; auto. *)
+      - unfold_pures.
+        autorewrite with sep.
+        rewrite H0 in HP.
+        rewrite nth_overflow; eauto.
+        rewrite distribute_length; auto.
+        (* destruct e as [|e]; [unfold_pures; cbv in HP2; inversion HP2|].   *)
+        (* change_; [intros Hf|]. *)
+        (* { autorewrite with sep in HP5; auto; unfold_pures. *)
+        (*   rewrite HP1 in n0; rewrite <-Nat2Z.inj_lt in n0. *)
+        (*   rewrite nth_overflow; [|rewrite distribute_length; autorewrite with sep in *; omega]. *)
+        (*   exact Hf. } *)
+        (* sep_combine_in H; sep_cancel; exact H. *) } Unfocus.
 
     (* loop invariant is preserved *)
-    instantiate (1 := INV (nf tid)); unfold INV; intros; apply ex_lift_l_in in H; destruct H as [s0 H].
+    instantiate (1 := INV2 (nf tid) (nf bid)); unfold INV2; intros; apply ex_lift_l_in in H; destruct H as [s0 H].
+    apply ex_lift_l_in in H; destruct H as [e0 H].
     apply ex_lift_l_in in H; destruct H as [fc' H].
     sep_split_in H.
     unfold_pures.
-    destruct e; [cbv in l; congruence|].
-    autorewrite with sep in *; auto.  clear HP3 HP7.
-    exists (2 ^ e / 2), e, fc'; sep_split; try now simpl; first [eauto | omega | congruence];
-    autorewrite with sep; auto.
-    + rewrite HP1 in n0; rewrite <-Nat2Z.inj_lt in n0; unfold_conn.
-      destruct e as [|e]; [destruct (lt_dec _ (ceil2 (_/_))) as [Hlt | ?]; unfold_conn; auto |].
-      unfold ceil2 in Hlt; simpl in n0, Hlt; omega.
+    (* destruct e; [cbv in l; congruence|]. *)
+    exists s0 e0 fc'.
+    sep_split; eauto.
+    unfold ceil2 in H; destruct Nat.eq_dec; eauto.
+    (* autorewrite with sep in *; auto.  clear HP3 HP7. *)
+    (* exists (2 ^ e / 2), e, fc'; sep_split; try now simpl; first [eauto | omega | congruence]; *)
+    (* autorewrite with sep; auto. *)
+    (* + rewrite HP1 in n0; rewrite <-Nat2Z.inj_lt in n0; unfold_conn. *)
+    (*   destruct e as [|e]; [destruct (lt_dec _ (ceil2 (_/_))) as [Hlt | ?]; unfold_conn; auto |]. *)
+    (*   unfold ceil2 in Hlt; simpl in n0, Hlt; omega. *)
 
-      autorewrite with sep; auto; simpl in *.
-      destruct lt_dec; [omega | unfold_conn; auto].
-    + unfold_conn; destruct e; [cbv; omega|autorewrite with sep; auto].
-      simpl in HP4; omega.
-    + cutrewrite (2%Z = Z.of_nat 2) in HP0; [|auto]; rewrite <-div_Zdiv in HP0; auto. simpl in HP0.
-      rewrite HP6 in HP0; apply Nat2Z.inj in HP0; subst.
-      destruct e; [unfold div, ceil2 in *; simpl in *; auto|].
-      autorewrite with sep in *; auto.
-      destruct Nat.eq_dec; [apply Nat.pow_nonzero in e0; auto; destruct e0|].
-      apply H.
+    (*   autorewrite with sep; auto; simpl in *. *)
+    (*   destruct lt_dec; [omega | unfold_conn; auto]. *)
+    (* + unfold_conn; destruct e; [cbv; omega|autorewrite with sep; auto]. *)
+    (*   simpl in HP4; omega. *)
+    (* + cutrewrite (2%Z = Z.of_nat 2) in HP0; [|auto]; rewrite <-div_Zdiv in HP0; auto. simpl in HP0. *)
+    (*   rewrite HP6 in HP0; apply Nat2Z.inj in HP0; subst. *)
+    (*   destruct e; [unfold div, ceil2 in *; simpl in *; auto|]. *)
+    (*   autorewrite with sep in *; auto. *)
+    (*   destruct Nat.eq_dec; [apply Nat.pow_nonzero in e0; auto; destruct e0|]. *)
+    (*   apply H. *)
   - unfold_conn; intros; tauto.
-  - intros s h H; unfold INV in *.
-    apply ex_lift_l_in in H; destruct H as [? H].
-    apply ex_lift_l_in in H; destruct H as [? H].
-    apply ex_lift_l_in in H; destruct H as [fc' H].
-    sep_split_in H.
-    assert (x = 0).
-    { unfold_conn_in (HP, HP1); simpl in HP, HP1; destruct Z_lt_dec; simpl in HP; try congruence.
-      rewrite HP1 in n0; cutrewrite (0%Z = Z.of_nat 0) in n0; [|auto]; rewrite <-Nat2Z.inj_lt in n0.
-      omega. }
-    subst; simpl in *.
-    exists fc'.
-    sep_split; auto.
-    destruct (Nat.eq_dec (nf tid) 0); [|cbv; tauto].
-    rewrite e in HP3; simpl in HP3; destruct HP3.
-    unfold dbl in H0; simpl in H0.
-    rewrite skip_sum_sum in H0. auto.
+  - intros; eauto.
+  - eapply Hforward.
+    + eapply rule_if_disj.
+      * eapply Hbackward.
+        Focus 2.
+        { intros s h H; unfold INV2 in *.
+          sep_split_in H.
+          sep_lift_in H 3.
+          apply ex_lift_l_in in H; destruct H as [s0 H].
+          apply ex_lift_l_in in H; destruct H as [e H].
+          apply ex_lift_l_in in H; destruct H as [fc' H].
+          sep_normal_in H; sep_split_in H.
+          assert (s0 = 0); [|subst s0].
+          { unfold_pures. nia. }
+          unfold dbl in *; simpl in *.
+          assert (Heq : nf tid = 0); [|rewrite Heq in *].
+          { unfold_pures; nia. }
+          unfold ceil2 in *; simpl in *.
+          rewrite skip_sum_sum in HP5.
+          lets unf: (>>(@skip_arr_unfold') 0 ntrd 1 0); eauto.
+          simpl in unf.
+          sep_rewrite_in unf H; eauto; clear unf.
+          destruct HP5 as [Heq' _]; rewrite Heq' in H.
+          assert (pure (nf tid = 0) s (emp_ph loc)) by (unfold_conn; auto).
+          assert (pure (fc' 0 = sum_of 0 ntrd f_ss) s (emp_ph loc)) by (unfold_conn; auto).
+          clear HP3 HP4 HP6; sep_combine_in H.
+          ex_intro fc' H; exact H. } Unfocus.
+        repeat hoare_forward.
+        eapply rule_seq.
+        hoare_forward; [intros ? ? H; exact H|..].
+        hoare_forward.
+        intros ? ? H. ex_intro x3 H; exact H.
+      * apply rule_skip.
+    + intros s h [H|H].
+      * destruct H as [fc' H].
+        exists fc'; sep_split_in H; sep_split; unfold_pures.
+        destruct Nat.eq_dec; try omega.
+        rewrite e0 in *; simpl.
+        repeat sep_cancel.
+        lets unf: (>>(@skip_arr_unfold') 0 ntrd 1 0); eauto.
+        simpl in unf.
+        sep_rewrite unf; eauto; clear unf.
+        rewrite HP5.
+        sep_normal; repeat sep_cancel.
+      * unfold INV2 in *; sep_split_in H.
+        sep_lift_in H 3.
+        apply ex_lift_l_in in H; destruct H as [s0 H].
+        apply ex_lift_l_in in H; destruct H as [e H].
+        apply ex_lift_l_in in H; destruct H as [fc' H].
+        sep_normal_in H; sep_split_in H; unfold_pures.
+        exists fc'.
+        sep_cancel.
+        assert (s0 = 0) by nia.
+        rewrite H1 in *; simpl in H0.
+        assert (nf tid <> 0) by nia.
+        destruct (Nat.eq_dec (nf tid)); try omega.
+        rewrite nth_overflow in H0; sep_normal_in H0; eauto.
+        rewrite distribute_length; nia.
 Qed.
-
   
 Definition ty_env_fold (v : var) :=
   if var_eq_dec v TID then Hi
